Most of lecture 2 translated

coq/Indexed.v
@@ -2,6 +2,8 @@
 
 Require Ascii String.
 From Equations Require Import Equations.
+Require FunctionalExtensionality.
+Require Import MPRICoq.Monad.
 
 (** **Typing `sprintf` *)
 Module sprintf.
@@ -37,15 +39,15 @@ Module sprintf.
     ⟦ (parse s) ⟧.
   Notation "⟦p s ⟧" := (parse_and_type s).
 
-  Fixpoint showNat (n : nat) : string :=
+  Fixpoint show_nat (n : nat) : string :=
     match n with
     | O => "O"
-    | S n => "S(" ++ (showNat n) ++ ")"
+    | S n => "S(" ++ (show_nat n) ++ ")"
     end.
 
   Fixpoint eval (fmt : format) (acc : string) : ⟦ fmt ⟧ :=
     match fmt return ⟦ fmt ⟧ with
-    | digitf k => fun n => eval k (acc ++ (showNat n))
+    | digitf k => fun n => eval k (acc ++ (show_nat n))
     | stringf k => fun s => eval k (acc ++ s)
     | symbf c k => eval k (acc ++ String c "")
     | endf => acc
@@ -136,7 +138,7 @@ Module NormalForms.
         mono_inter (weak2 wk) (suc k) := suc (mono_inter wk k) }.
     Notation "⟦ wk ⟧" := (mono_inter wk).
 
-    (* TODO What ? *)
+    (* TODO *)
     (* Lemma lemma_valid : forall m n k l (wk : m ⊇ n), k <= l -> ⟦ wk ⟧ k <= ⟦ wk ⟧ l. *)
   End Fin.
 
@@ -163,11 +165,6 @@ Module NormalForms.
       rename wk (pair a b) := pair (rename wk a) (rename wk b);
       rename wk (fst p) := fst (rename wk p);
       rename wk (snd p) := snd (rename wk p) }.
-
-  (* Definition rename_lam {Γ Δ t} : (t ∈ Γ) -> (forall {s}, s ∈ Γ -> Δ ⊢ s) -> Δ ⊢ t. *)
-  (* Admitted. *)
-  (*   (* rename_lam here _ := var here; *) *)
-  (*   (* rename_lam (there v) ρ := rename (weak1 id) (ρ _ v). *) *)
 
   (* Equations sub {Γ Δ t}: (Γ ⊢ t) -> (forall {s}, s ∈ Γ -> Δ ⊢ s) -> Δ ⊢ t := *)
   (*   { sub (lam t) ρ := lam (sub t (fun s H  with H := *)
@@ -262,97 +259,421 @@ Module NormalForms.
   Admitted.
 
   (** **Normal forms *)
+  Module Model1.
 
-  (** We can represent the equation theory as an inductive family: *)
-  (* Reserved Notation "Γ ⊢ T ∋ t ⤳ s" (at level 70). *)
-  Inductive βη_norm : forall (Γ : context) (T : type), Γ ⊢ T -> Γ ⊢ T -> Prop :=
-  | rule_β : forall{Γ T S}{b : Γ ▷ S ⊢ T}{s : Γ ⊢ S},
-      βη_norm Γ T (app (lam b) s) (sub1 b s)
-  | rule_η_fun : forall{Γ T S}{f : Γ ⊢ S ⇒ T},
-      βη_norm Γ (S ⇒ T) f (lam (app (rename (weak1 id) f) (var here)))
-  | rule_η_pair : forall{Γ A B}{p : Γ ⊢ A × B},
-      βη_norm Γ (A × B) p (pair (fst p) (snd p)).
+    (** We can represent the equation theory as an inductive family: *)
+    (* Reserved Notation "Γ ⊢ T ∋ t ⤳ s" (at level 70). *)
+    Inductive βη_norm : forall (Γ : context) (T : type), Γ ⊢ T -> Γ ⊢ T -> Prop :=
+    | rule_β : forall{Γ T S}{b : Γ ▷ S ⊢ T}{s : Γ ⊢ S},
+        βη_norm Γ T (app (lam b) s) (sub1 b s)
+    | rule_η_fun : forall{Γ T S}{f : Γ ⊢ S ⇒ T},
+        βη_norm Γ (S ⇒ T) f (lam (app (rename (weak1 id) f) (var here)))
+    | rule_η_pair : forall{Γ A B}{p : Γ ⊢ A × B},
+        βη_norm Γ (A × B) p (pair (fst p) (snd p)).
+    
+    Inductive βη_eq : forall (Γ : context) (T : type), Γ ⊢ T -> Γ ⊢ T -> Prop :=
+    | inc : forall {Γ T t1 t2},
+        βη_norm Γ T t1 t2 ->
+        βη_eq Γ T t1 t2
+    | refl : forall {Γ T t},
+        βη_eq Γ T t t
+    | sym : forall {Γ T t1 t2},
+        βη_eq Γ T t1 t2 ->
+        βη_eq Γ T t2 t1
+    | trans : forall {Γ T t1 t2 t3},
+        βη_eq Γ T t1 t2 -> βη_eq Γ T t2 t3 ->
+        βη_eq Γ T t1 t3
+    | struct_lam : forall{Γ S T b b'},
+        βη_eq (Γ ▷ S) T b b' ->
+        βη_eq Γ (S ⇒ T) (lam b) (lam b')
+    | struct_app : forall{Γ S T f f' s s'},
+        βη_eq Γ (S ⇒ T) f f' -> βη_eq Γ S s s' ->
+        βη_eq Γ T (app f s) (app f' s')
+    | struct_pair : forall{Γ A B a a' b b'},
+        βη_eq Γ A a a' -> βη_eq Γ B b b' ->
+        βη_eq Γ (A × B) (pair a b) (pair a' b')
+    | struct_fst : forall{Γ A B p p'},
+        βη_eq Γ (A × B) p p' ->
+        βη_eq Γ A (fst p) (fst p')
+    | struct_snd : forall{Γ A B p p'},
+        βη_eq Γ (A × B) p p' ->
+        βη_eq Γ B (snd p) (snd p').
 
-  Inductive βη_eq : forall (Γ : context) (T : type), Γ ⊢ T -> Γ ⊢ T -> Prop :=
-  | inc : forall {Γ T t1 t2},
-      βη_norm Γ T t1 t2 ->
-      βη_eq Γ T t1 t2
-  | refl : forall {Γ T t},
-      βη_eq Γ T t t
-  | sym : forall {Γ T t1 t2},
-      βη_eq Γ T t1 t2 ->
-      βη_eq Γ T t2 t1
-  | trans : forall {Γ T t1 t2 t3},
-      βη_eq Γ T t1 t2 -> βη_eq Γ T t2 t3 ->
-      βη_eq Γ T t1 t3
-  | struct_lam : forall{Γ S T b b'},
-      βη_eq (Γ ▷ S) T b b' ->
-      βη_eq Γ (S ⇒ T) (lam b) (lam b')
-  | struct_app : forall{Γ S T f f' s s'},
-      βη_eq Γ (S ⇒ T) f f' -> βη_eq Γ S s s' ->
-      βη_eq Γ T (app f s) (app f' s')
-  | struct_pair : forall{Γ A B a a' b b'},
-      βη_eq Γ A a a' -> βη_eq Γ B b b' ->
-      βη_eq Γ (A × B) (pair a b) (pair a' b')
-  | struct_fst : forall{Γ A B p p'},
-      βη_eq Γ (A × B) p p' ->
-      βη_eq Γ A (fst p) (fst p')
-  | struct_snd : forall{Γ A B p p'},
-      βη_eq Γ (A × B) p p' ->
-      βη_eq Γ B (snd p) (snd p').
+    (** ***Compute η-long β-normal forms for the simply typed λ-calculus: *)
+    Inductive term : Type :=
+    | Lam (v : String.string) (b : term) : term
+    | Var (v : String.string) : term
+    | App (f s : term) : term
+    | Tt : term
+    | Pair (a b : term) : term
+    | Fst (p : term) : term
+    | Snd (p : term) : term.
 
-  (** ***Compute η-long β-normal forms for the simply typed λ-calculus: *)
-  Inductive term : Type :=
-  | Lam (v : String.string) (b : term) : term
-  | Var (v : String.string) : term
-  | App (f s : term) : term
-  | Tt : term
-  | Pair (a b : term) : term
-  | Fst (p : term) : term
-  | Snd (p : term) : term.
+    Reserved Notation "⟦ T ⟧Type".
+    Fixpoint interp_type (T : type) : Type :=
+      match T with
+      | unit => term
+      | T1 ⇒ T2 => ⟦ T1 ⟧Type -> ⟦ T2 ⟧Type
+      | T1 × T2 => ⟦ T1 ⟧Type * ⟦ T2 ⟧Type
+      end
+    where "⟦ T ⟧Type" := (interp_type T).
 
-  Reserved Notation "⟦ T ⟧Type".
-  Fixpoint interp_type (T : type) : Type :=
-    match T with
-    | unit => term
-    | T1 ⇒ T2 => ⟦ T1 ⟧Type -> ⟦ T2 ⟧Type
-    | T1 × T2 => ⟦ T1 ⟧Type * ⟦ T2 ⟧Type
-    end
-  where "⟦ T ⟧Type" := (interp_type T).
+    Reserved Notation "⟦ Γ ⟧context".
+    Fixpoint interp_context (Γ : context) : Type :=
+      match Γ with
+      | ϵ => Datatypes.unit
+      | Γ ▷ T1 => ⟦ Γ ⟧context * ⟦ T1 ⟧Type
+      end
+    where "⟦ Γ ⟧context" := (interp_context Γ).
 
-  Reserved Notation "⟦ Γ ⟧context".
-  Fixpoint interp_context (Γ : context) : Type :=
-    match Γ with
-    | ϵ => Datatypes.unit
-    | Γ ▷ T1 => ⟦ Γ ⟧context * ⟦ T1 ⟧Type
-    end
-  where "⟦ Γ ⟧context" := (interp_context Γ).
+    Definition interp_type_context (Γ : context) (T : type) : Type :=
+      ⟦ Γ ⟧context -> ⟦ T ⟧Type.
+    Notation "Γ ⊩ T" := (interp_type_context Γ T) (at level 50).
 
-  Definition interp_type_context (Γ : context) (T : type) : Type :=
-    ⟦ Γ ⟧context -> ⟦ T ⟧Type.
-  Notation "Γ ⊩ T" := (interp_type_context Γ T) (at level 50).
+    Fixpoint lookup {Γ T} (v : T ∈ Γ) : Γ ⊩ T :=
+      match v with
+      | here => fun '(_, x) => x
+      | there h => fun '(γ, _) => lookup h γ
+      end.
 
-  Fixpoint lookup {Γ T} (v : T ∈ Γ) : Γ ⊩ T :=
-    match v with
-    | here => fun '(_, x) => x
-    | there h => fun '(γ, _) => lookup h γ
-    end.
+    Fixpoint eval {Γ T} (t : Γ ⊢ T) : Γ ⊩ T :=
+      match t with
+      | var v => fun ρ => lookup v ρ
+      | app f s => fun ρ => eval f ρ (eval s ρ)
+      | lam b => fun ρ => fun s => eval b (ρ, s)
+      | pair a b => fun ρ => (eval a ρ , eval b ρ)
+      | fst p => fun ρ => Datatypes.fst (eval p ρ)
+      | snd p => fun ρ => Datatypes.snd (eval p ρ)
+      | tt => fun _ => Tt
+      end.
 
-  Fixpoint eval {Γ T} (t : Γ ⊢ T) : Γ ⊩ T :=
-    match t with
-    | var v => fun ρ => lookup v ρ
-    | app f s => fun ρ => eval f ρ (eval s ρ)
-    | lam b => fun ρ => fun s => eval b (ρ, s)
-    | pair a b => fun ρ => (eval a ρ , eval b ρ)
-    | fst p => fun ρ => Datatypes.fst (eval p ρ)
-    | snd p => fun ρ => Datatypes.snd (eval p ρ)
-    | tt => fun _ => Tt
-    end.
-
-  (** Let us, for simplicity, assume that we have access to a fresh name
+    (** Let us, for simplicity, assume that we have access to a fresh name
       generator, `gensym` *)
-  Axiom gensym : Datatypes.unit -> String.string.
+    Axiom gensym : Datatypes.unit -> String.string.
 
-  (* TODO *)
+    (** We could then back-translate the objects in the model (`⟦_⟧Type`)
+      back to raw terms (through `reify`). However, to do so, one needs to
+      inject variables in η-long normal form into the model: this is the
+      role of `reflect`: *)
+    Equations reify (T : type) : ⟦ T ⟧Type -> term :=
+      { reify unit t => t;
+        reify (T1 ⇒ T2) t => let freshx := gensym Datatypes.tt in
+                            Lam freshx (reify T2 (t (reflect T1 (Var freshx))));
+        reify (T1 × T2) (f, s) => Pair (reify T1 f) (reify T2 s)
+      } with reflect (T : type) : term -> ⟦ T ⟧Type :=
+        { reflect unit t => t;
+          reflect (T1 ⇒ T2) t => fun s => reflect T2 (App t (reify T1 s));
+          reflect (T1 × T2) t => (reflect T1 (Fst t), reflect T2 (Snd t))
+        }.
 
+    (** Given a λ-term, we can thus compute its normal form: *)
+    Fixpoint idC (Γ : context) : ⟦ Γ ⟧context :=
+      match Γ with
+      | ϵ => Datatypes.tt
+      | (Γ ▷ T) => (idC Γ, reflect T (Var (gensym Datatypes.tt)))
+      end.
+    Definition norm {Γ T} Δ := reify T (eval Δ (idC Γ)).
+
+    (** Just like in the previous lecture, we can use it to check whether any two
+      terms belong to the same congruence class by comparing their normal forms *)
+    Definition term1 : ϵ ⊢ (unit ⇒ unit) ⇒ (unit ⇒ unit) :=
+      (* λ s. λ z. s (s z) *)
+      lam (lam (app (var (there here)) (app (var (there here)) (var here)))).
+
+    Definition term2 : ϵ ⊢ (unit ⇒ unit) ⇒ (unit ⇒ unit) :=
+      (* λ s. (λ r. λ z. r (s z)) (λ x. s x) *)
+      lam (app (lam (lam (app (var (there here))
+                              (app (var (there (there here))) (var here)))))
+               (lam (app (var (there here)) (var here)))).
+
+    Example test_nbe : norm term1 = norm term2.
+    Proof. reflexivity. Qed.
+
+    (** For instance, thanks to a suitable model construction, we have
+      surjective pairing *)
+    Definition term3 : ϵ ⊢ (unit × unit) ⇒ (unit × unit) :=
+      (* λ p. p *)
+      lam (var here).
+
+    Definition term4 : ϵ ⊢ (unit × unit) ⇒ (unit × unit) :=
+      (* λ p. (fst p, snd p) *)
+      lam (pair (fst (var here)) (snd (var here))).
+
+    Example test_nbe2 : norm term3 = norm term4.
+    Proof. reflexivity. Qed.
+
+    (** However, this implementation is a bit of wishful thinking: we do not
+      have a `gensym`! So the following is also true, for the bad reason
+      that `gensym` is not actually producing unique names but always the
+      same name (itself): *)
+    Definition term5 : ϵ ⊢ unit ⇒ (unit ⇒ unit) :=
+      (* λ z1 z2. z1 *)
+      lam (lam (var (there here))).
+
+    Definition term6 : ϵ ⊢ unit ⇒ (unit ⇒ unit) :=
+      (* λ z1 z2. z2 *)
+      lam (lam (var here)).
+
+    Example test_nbe3 : norm term5 = norm term6.
+    Proof. reflexivity. Qed. (* BUG ! *)
+  End Model1.
+
+  (** This might not deter the brave monadic programmer: we can emulate
+      `gensym` using a reenactment of the state monad: *)
+  Module Fresh.
+    Import FunctionalExtensionality.
+
+    Definition Fresh (A : Type) : Type := nat -> (A * nat).
+    Definition gensym (tt : Datatypes.unit) : Fresh String.string :=
+      fun n => (sprintf.show_nat n, 1 + n).
+
+    Program Instance FreshMonad : Monad Fresh :=
+      {
+        ret _ x := fun n => (x, n);
+        bind _ _ x k := fun n => let (a, n') := x n in k a n'
+      }.
+    Next Obligation.
+      apply functional_extensionality; intro n.
+      destruct (x n) as [a n']. reflexivity.
+    Qed.
+    Next Obligation.
+      apply functional_extensionality; intro n.
+      destruct (x n) as [a n'].
+      destruct (f a n') as [a1 n1].
+      reflexivity.
+    Qed.
+
+  (** We then simply translate the previous code to a monadic style, a
+      computer could do it automatically: *)
+    (* Equations reify (T : type) : ⟦ T ⟧Type -> Fresh term := *)
+    (*   { reify unit t => ret t; *)
+    (*     reify (T1 × T2) (a, b) => *)
+    (*     reify T1 a >>= *)
+    (*           fun a => reify T2 b >>= *)
+    (*                       fun b => ret (Pair a b); *)
+    (*     reify (T1 ⇒ T2) f => *)
+    (*     gensym Datatypes.tt >>= *)
+    (*            fun s => reflect T1 (Var s) >>= *)
+    (*                          fun t => reify T2 (f t) >>= *)
+    (*                                      fun b => ret (Lam s b) *)
+    (*   } with reflect (T : type) : term -> Fresh ⟦ T ⟧Type := *)
+    (*     { reflect unit t => ret t; *)
+    (*       reflect (T1 × T2) t => *)
+    (*       reflect T1 (Fst t) >>= *)
+    (*               fun a => reflect T2 (Snd t) >>= *)
+    (*                             fun b => ret (a, b); *)
+    (*       reflect (T1 ⇒ T2) t => ret (fun s => _) *)
+    (*     }. *)
+    (* cannot conclude with `reflect T (neu ! reify s)` *)
+  End Fresh.
+
+  (** **The Rising Sea *)
+  Module Model2.
+
+    Reserved Notation "Γ ⊢Nf T" (at level 50).
+    Reserved Notation "Γ ⊢Ne T" (at level 50).
+    Inductive has_type_nf (Γ : context) : type -> Type :=
+    | Lam {S T} (b : Γ ▷ S ⊢Nf T) : Γ ⊢Nf S ⇒ T
+    | Pair {A B} (a : Γ ⊢Nf A) (b : Γ ⊢Nf B) : Γ ⊢Nf A × B
+    | Tt : Γ ⊢Nf unit
+    | Ground (grnd : Γ ⊢Ne unit) : Γ ⊢Nf unit
+    where "Γ ⊢Nf T" := (has_type_nf Γ T)
+    with has_type_ne (Γ : context) : type -> Type :=
+         | Var {T} (v : T ∈ Γ) : Γ ⊢Ne T
+         | App {S T} (f : Γ ⊢Ne S ⇒ T) (s : Γ ⊢Nf S) : Γ ⊢Ne T
+         | Fst {A B} (p : Γ ⊢Ne A × B) : Γ ⊢Ne A
+         | Snd {A B} (p : Γ ⊢Ne A × B) : Γ ⊢Ne B
+    where "Γ ⊢Ne T" := (has_type_ne Γ T).
+    Arguments Lam {_ _ _}. Arguments App {_ _ _}.
+    Arguments Tt {_}. Arguments Ground {_}. Arguments Var {_ _}.
+    Arguments Fst {_ _ _}. Arguments Snd {_ _ _}. Arguments Pair {_ _ _}.
+
+    Reserved Notation "⎣ t ⎦Nf".
+    Reserved Notation "⎣ t ⎦Ne".
+    Fixpoint nf_to_term {Γ T} (t : Γ ⊢Nf T) : Γ ⊢ T :=
+      match t with
+      | Lam b => lam ⎣ b ⎦Nf
+      | Ground grnd => ⎣ grnd ⎦Ne
+      | Pair a b => pair ⎣ a ⎦Nf ⎣ b ⎦Nf
+      | Tt => tt
+      end
+    where "⎣ t ⎦Nf" := (nf_to_term t)
+    with ne_to_term {Γ T} (t : Γ ⊢Ne T) : Γ ⊢ T :=
+           match t with
+           | Var v => var v
+           | App f s => app ⎣ f ⎦Ne ⎣ s ⎦Nf
+           | Fst p => fst ⎣ p ⎦Ne
+           | Snd p => snd ⎣ p ⎦Ne
+           end
+    where "⎣ t ⎦Ne" := (ne_to_term t).
+
+    Class Sem : Type :=
+      { sem_context : context -> Type;
+        ren {Γ Δ} : Γ ⊇ Δ -> sem_context Δ -> sem_context Γ
+      }.
+
+    Local Set Warnings "-implicits".
+    Definition context_and_type (P Q : Sem) : Type :=
+      forall {Γ}, @sem_context P Γ -> @sem_context Q Γ.
+    Notation "P ⟦⊢⟧ Q" := (context_and_type P Q) (at level 80).
+
+    Fixpoint rename_Nf {Γ Δ T} (wk : Γ ⊇ Δ) (t : Δ ⊢Nf T) : Γ ⊢Nf T :=
+      match t with
+      | Lam b => Lam (rename_Nf (weak2 wk) b)
+      | Ground grnd => Ground (rename_Ne wk grnd)
+      | Pair a b => Pair (rename_Nf wk a) (rename_Nf wk b)
+      | Tt => Tt
+      end
+    with rename_Ne {Γ Δ T} (wk : Γ ⊇ Δ) (t : Δ ⊢Ne T) : Γ ⊢Ne T :=
+           match t with
+           | Var v => Var (shift wk v)
+           | App f s => App (rename_Ne wk f) (rename_Nf wk s)
+           | Fst p => Fst (rename_Ne wk p)
+           | Snd p => Snd (rename_Ne wk p)
+           end.
+
+    Instance Nf (T : type) : Sem :=
+      { sem_context Γ := Γ ⊢Nf T;
+        ren _ _ := rename_Nf }.
+
+    Instance Ne (T : type) : Sem :=
+      { sem_context Γ := Γ ⊢Ne T;
+        ren _ _ := rename_Ne }.
+
+    (** Following our earlier model, we will interpret the `unit` type as
+        the normal forms of type `unit`: *)
+    Definition sem_unit : Sem := Nf unit.
+    Notation "⟦unit⟧" := sem_unit.
+
+    Definition sem_tt {P} : P ⟦⊢⟧ ⟦unit⟧ := fun _ _ => Tt.
+    Notation "⟦tt⟧" := sem_tt.
+
+    (** Similarly, we will interpret the `_×_` type as a product in
+        `Sem`, defined in a pointwise manner: *)
+    Instance sem_prod (P Q : Sem) : Sem :=
+      { sem_context Γ := Datatypes.prod (@sem_context P Γ) (@sem_context Q Γ);
+        ren _ _ wk '(x, y) := (@ren P _ _ wk x, @ren Q _ _ wk y) }.
+    Notation "P ⟦×⟧ Q" := (sem_prod P Q) (at level 70).
+
+    Definition sem_pair {P Q R} : P ⟦⊢⟧ Q -> P ⟦⊢⟧ R -> P ⟦⊢⟧ Q ⟦×⟧ R :=
+      fun a b ρ Γ => (a ρ Γ, b ρ Γ).
+    Notation "⟦pair⟧" := sem_pair.
+
+    Definition sem_fst {P Q R} : P ⟦⊢⟧ Q ⟦×⟧ R -> P ⟦⊢⟧ Q :=
+      fun p ρ Γ => Datatypes.fst (p ρ Γ).
+    Notation "⟦fst⟧" := sem_fst.
+
+    Definition sem_snd {P Q R} : P ⟦⊢⟧ Q ⟦×⟧ R -> P ⟦⊢⟧ R :=
+      fun p ρ Γ => Datatypes.snd (p ρ Γ).
+    Notation "⟦snd⟧" := sem_snd.
+
+    (** ***Interlude: Yoneda lemma *)
+    (* TODO *)
+
+    (** ***Back to the Sea *)
+    Instance sem_arrow (P Q : Sem) : Sem :=
+      { sem_context Γ := forall {Δ}, Δ ⊇ Γ -> @sem_context P Δ -> @sem_context Q Δ;
+        ren _ _ wk1 k _ wk2 := k _ (wk1 ∘wk wk2) }.
+    Notation "P ⟦⇒⟧ Q" := (sem_arrow P Q) (at level 70).
+
+    Definition sem_lam {P Q R} : P ⟦×⟧ Q ⟦⊢⟧ R -> P ⟦⊢⟧ Q ⟦⇒⟧ R :=
+      fun η _ p _ wk q => η _ (ren wk p , q).
+    Notation "⟦lam⟧" := sem_lam.
+
+    Definition sem_app {P Q R} : P ⟦⊢⟧ Q ⟦⇒⟧ R -> P ⟦⊢⟧ Q -> P ⟦⊢⟧ R :=
+      fun η μ _ px => η _ px _ id (μ _ px).
+    Notation "⟦app⟧" := sem_app.
+
+    (** At this stage, we have enough structure to interpret the types *)
+    Reserved Notation "⟦ T ⟧".
+    Fixpoint interp_type (T : type) : Sem :=
+      match T with
+      | unit => ⟦unit⟧
+      | T1 ⇒ T2 => ⟦ T1 ⟧ ⟦⇒⟧ ⟦ T2 ⟧
+      | T1 × T2 => ⟦ T1 ⟧ ⟦×⟧ ⟦ T2 ⟧
+      end
+    where "⟦ T ⟧" := (interp_type T).
+
+    (** To interpret contexts, we also need a terminal object: *)
+    Instance terminal : Sem :=
+      { sem_context _ := Datatypes.unit;
+        ren _ _ _ _ := Datatypes.tt }.
+    Notation "⟦⊤⟧" := terminal.
+
+    Reserved Notation "⟦ Γ ⟧C".
+    Fixpoint interp_context (Γ : context) : Sem :=
+      match Γ with
+      | ϵ => ⟦⊤⟧
+      | Γ ▷ T => ⟦ Γ ⟧C ⟦×⟧ ⟦ T ⟧
+      end
+    where "⟦ Γ ⟧C" := (interp_context Γ).
+
+    (** As usual, a type in context will be interpreted as a morphism between
+        their respective interpretations. The interpreter then takes the
+        syntactic object to its semantical counterpart: *)
+    Definition sem_has_type (Γ : context) (T : type) : Type :=
+      ⟦ Γ ⟧C ⟦⊢⟧ ⟦ T ⟧.
+    Notation "Γ ⊩ T" := (sem_has_type Γ T) (at level 80).
+
+    Fixpoint lookup {Γ T} (v : T ∈ Γ) : Γ ⊩ T :=
+      match v with
+      | here => fun _ '(_, v) => v
+      | there x => fun _ '(γ, _) => lookup x _ γ
+      end.
+
+    Fixpoint eval {Γ T} (t : Γ ⊢ T) : Γ ⊩ T :=
+      match t with
+      | lam b => ⟦lam⟧ (eval b)
+      | var v => lookup v
+      | app f s => ⟦app⟧ (eval f) (eval s)
+      | tt => ⟦tt⟧
+      | pair a b => ⟦pair⟧ (eval a) (eval b)
+      | fst p => ⟦fst⟧ (eval p)
+      | snd p => ⟦snd⟧ (eval p)
+      end.
+
+    (** Reify and reflect are defined for a given syntactic context, we
+        therefore introduce suitable notations: *)
+
+    Definition synt_has_type (Γ : context) (T : type) : Type :=
+      @sem_context ⟦T⟧ Γ.
+    Notation "[ Γ ]⊩ T" := (synt_has_type Γ T) (at level 80).
+
+    Definition synt_has_context (Γ Δ : context) : Type :=
+      @sem_context ⟦Δ⟧C Γ.
+    Notation "[ Γ ]⊩C Δ" := (synt_has_context Γ Δ) (at level 80).
+
+    (** The sea has sufficiently risen: we can implement our initial plan,
+        using the renaming operator `ren` equipping `Sem` in the function
+        case in `reify`: *)
+
+    Fixpoint reify {Γ} (T : type) : [ Γ ]⊩ T -> Γ ⊢Nf T :=
+      match T with
+      | unit => fun v => v
+      | T1 ⇒ T2 =>
+        fun f => Lam (reify T2 ((ren (weak1 id) f) _ id (reflect T1 (Var here))))
+      | A × B => fun '(a, b) => Pair (reify A a) (reify B b)
+      end
+    with reflect {Γ} (T : type) : Γ ⊢Ne T -> [ Γ ]⊩ T :=
+           match T with
+           | unit => Ground
+           | T1 ⇒ T2 =>
+             fun v _ w s => reflect T2 (App (@ren (Ne _) _ _ w v) (reify T1 s))
+           | A × B => fun v => (reflect A (Fst v), reflect B (Snd v))
+           end.
+
+    Fixpoint idC (Γ : context) : [ Γ ]⊩C Γ :=
+      match Γ with
+      | ϵ => Datatypes.tt
+      | (Γ ▷ T) => (ren (weak1 id) (idC Γ), reflect T (Var here))
+      end.
+    Definition reify_id {Γ T} (f : Γ ⊩ T) : Γ ⊢Nf T :=
+      reify _ (f _ (idC Γ)).
+
+    Definition norm {Γ T} (t : Γ ⊢ T) : Γ ⊢Nf T :=
+      reify_id (eval t).
+  End Model2.
 End NormalForms.
+
+(** **Optional: Categorical spotting *)
+(* TODO *)
